drafts/StreamExecution.v
@@ -1,0 +1,112 @@
+Section StreamExecution.
+
+  Variable H: history.
+  Variable arbitrary : stream.
+
+  Definition const_eqb (c1: const) (c2: const) : bool :=
+    match (c1, c2) with
+    | (Cint z1, Cint z2) => BinInt.Z.eqb z1 z2
+    | (Cbool b1, Cbool b2) => Bool.eqb b1 b2
+    | _ => false
+    end.
+
+  Definition value_eqb (v1: value) (v2: value) : bool :=
+    match (v1, v2) with
+    | (present c1, present c2) => const_eqb c1 c2
+    | (absent, absent) => true
+    | _ => false
+    end.
+
+  Fixpoint str_clock (ck: clock) (n: nat) : bool :=
+    match ck with
+    | Cbase => true
+    | Con ck' x c => match PM.find x H with
+                     | None => false
+                     | Some xs => andb (str_clock ck' n)
+                                       (value_eqb (xs n) (present (Cbool c)))
+                     end
+    end.
+
+  Fixpoint str_lexp (e: lexp) (n: nat) : value :=
+    match e with
+    | Econst c => present c
+    | Evar x => match PM.find x H with
+                | Some xs => xs n
+                | None => absent
+                end
+    | Ewhen e' x c => match PM.find x H with
+                      | Some xs => match xs n with
+                                   | present (Cbool b) =>
+                                     if Bool.eqb b c
+                                     then str_laexp e' n
+                                     else absent
+                                   | _ => absent
+                                   end
+                      | None => absent
+                      end
+    end
+  with str_laexp (e: laexp) (n: nat) : value :=
+    match e with
+    | LAexp ck e => if str_clock ck n then str_lexp e n else absent
+    end.
+
+  Lemma str_clock_spec:
+    forall ck n c,
+      sem_clock H ck n c
+      -> str_clock ck n = c.
+  Proof.
+    induction ck.
+    inversion 1; intuition.
+    intros n c.
+    inversion_clear 1;
+      repeat progress (simpl;
+         match goal with
+         | H:sem_var _ _ _ _ |- _ => inversion_clear H
+         | H: PM.find _ _ = _ |- _ => rewrite H
+         | H: _ = present (Cbool ?b) |- _ => (rewrite H; destruct b)
+         | H: sem_clock _ _ _ _ |- _ => (apply IHck in H; rewrite H)
+         | H: b <> _ |- _ => (apply Bool.not_true_is_false in H
+                              || apply Bool.not_false_is_true in H;
+                              rewrite H)
+         | _ => (cbv; reflexivity)
+         end).
+    destruct (PM.find i H); cbv; reflexivity.
+  Qed.
+
+  Lemma str_lexp_spec:
+    forall e n v,
+      sem_lexp H e n v
+      -> str_lexp e n = v.
+  Proof.
+    induction e using lexp_mult
+    with (P:=fun e => forall n v, sem_laexp H e n v -> str_laexp e n = v);
+    inversion 1;
+    repeat progress (simpl;
+           match goal with
+           | H:sem_lexp _ _ _ _ |- _ => (apply IHe in H; rewrite H)
+           | H:sem_laexp _ _ _ _ |- _ => (apply IHe in H; rewrite H)
+           | H:sem_clock _ _ _ _ |- _ => (apply str_clock_spec in H; rewrite H)
+           | H:sem_var _ _ _ _ |- _ => (inversion_clear H as [xs Hfind Hxsn];
+                                        rewrite Hfind; rewrite Hxsn)
+           | |- (if Bool.eqb ?b1 ?b2 then _ else _) = _ =>
+             try destruct b1; try destruct b2; simpl; intuition
+           | _ => intuition
+           end).
+  Qed.
+
+  Lemma str_laexp_spec:
+    forall e n v,
+      sem_laexp H e n v
+      -> str_laexp e n = v.
+  Proof.
+    inversion_clear 1; simpl;
+    repeat progress
+           match goal with
+           | H:sem_clock _ _ _ _ |- _ => (apply str_clock_spec in H; rewrite H)
+           | H:sem_lexp _ _ _ _ |- _ => (apply str_lexp_spec in H; rewrite H)
+           | _ => intuition
+           end.
+  Qed.
+
+End StreamExecution.
+
